type_system/wf_lemmas.v
@@ -1,12 +1,11 @@
-(* Add LoadPath "C:\Users\Ziga\Documents\Ziga_podatki\repositories\eeff-formalization\syntax". *)
-(* Add LoadPath "C:\Users\Ziga\Documents\Ziga_podatki\repositories\eeff-formalization\type_system". *)
-(* Add LoadPath "C:\Users\Ziga\Documents\Ziga_podatki\repositories\eeff-formalization\substitution". *)
-Add LoadPath "E:\Ziga_Podatki\faks\eeff-formalization\syntax".
-Add LoadPath "E:\Ziga_Podatki\faks\eeff-formalization\type_system".
-Add LoadPath "E:\Ziga_Podatki\faks\eeff-formalization\substitution".
+Add LoadPath "???\syntax".
+Add LoadPath "???\type_system".
+Add LoadPath "???\substitution".
 
 Require Export syntax_lemmas declarational.
 
+
+(* ==================== Types ==================== *)
 
 Lemma get_vtype_wf Γ num A : 
     wf_ctx Γ -> get_vtype Γ num = Some A -> wf_vtype A.
@@ -16,6 +15,37 @@ intros wf. revert num. induction wf; intros num gets; simpl in *.
 + destruct num. inv gets. auto. eauto.
 Qed.
 
+Lemma get_op_type_wf Σ op A_op B_op:
+  wf_sig Σ -> get_op_type Σ op = Some (A_op, B_op) ->
+  wf_vtype A_op /\ wf_vtype B_op.
+Proof.
+induction Σ; intros orig gets; constructor; simpl in *; try discriminate.
+all: destruct (op == o); inv orig; try inv gets; auto; apply IHΣ; auto.
+Qed.
+
+Lemma has_eq_wf_parts E Σ Γ Z T1 T2:
+  wf_eqs E Σ -> has_eq E Γ Z T1 T2 ->
+  wf_ctx Γ /\ wf_tctx Z /\ wf_t Γ Z T1 Σ /\ wf_t Γ Z T2 Σ.
+Proof.
+intros wf_eqs has. induction wf_eqs; inv has; auto.
+destruct H4 as [a [b [c d]]]. subst. do 3 aconstructor.  
+Qed.
+
+
+Fixpoint wf_sig_unique_cases Γ h Σ D op {struct Σ}:
+  has_htype Γ h Σ D -> get_op_type Σ op = None ->
+  get_case h op = None.
+Proof.
+intros htys gets.
+destruct Σ.
++ inv htys. inv H2. simpl. auto.
++ inv htys. inv H2. simpl in *.
+  destruct (op==o). discriminate.
+  eapply wf_sig_unique_cases; eauto.
+Qed.
+
+
+(* ==================== Contexts ==================== *)
 
 Lemma wf_ctx_insert Γ A i:
   wf_ctx Γ -> wf_vtype A -> wf_ctx (ctx_insert Γ i A).
@@ -40,15 +70,6 @@ Proof.
 revert i. induction Γ; intros i wf safe; simpl in *.
 + destruct i. inv wf. auto. omega.
 + destruct i. inv wf. auto. inv wf. eapply IHΓ; eauto. omega.
-Qed.
-
-
-Lemma get_op_type_wf Σ op A_op B_op:
-  wf_sig Σ -> get_op_type Σ op = Some (A_op, B_op) ->
-  wf_vtype A_op /\ wf_vtype B_op.
-Proof.
-induction Σ; intros orig gets; constructor; simpl in *; try discriminate.
-all: destruct (op == o); inv orig; try inv gets; auto; apply IHΣ; auto.
 Qed.
 
 
@@ -84,27 +105,6 @@ intros orig. induction Z; simpl in *. apply WfTCtxØ.
 inv orig. inv H2. apply WfTCtxU; auto.
 Qed.
 
-
-Lemma has_eq_wf_parts E Σ Γ Z T1 T2:
-  wf_eqs E Σ -> has_eq E Γ Z T1 T2 ->
-  wf_ctx Γ /\ wf_tctx Z /\ wf_t Γ Z T1 Σ /\ wf_t Γ Z T2 Σ.
-Proof.
-intros wf_eqs has. induction wf_eqs; inv has; auto.
-destruct H4 as [a [b [c d]]]. subst. do 3 aconstructor.  
-Qed.
-
-
-Fixpoint wf_sig_unique_cases Γ h Σ D op {struct Σ}:
-  has_htype Γ h Σ D -> get_op_type Σ op = None ->
-  get_case h op = None.
-Proof.
-intros htys gets.
-destruct Σ.
-+ inv htys. inv H2. simpl. auto.
-+ inv htys. inv H2. simpl in *.
-  destruct (op==o). discriminate.
-  eapply wf_sig_unique_cases; eauto.
-Qed.
 
 (* ==================== Instantiations ==================== *)
 
