README.md
@@ -2,7 +2,35 @@
 
 This repository contains the formalisation of the programming language EEFF.
 
-The three available branches are
-- master: contains the formalisation of EEFF with predicate logic
-- equational-logic: contains the formalisation of EEFF with equational logic
-- bidirectional: contains the formalisation of the bidirectional type inference
+The three branches are
+- *master*: contains the formalisation of EEFF with predicate logic
+- *equational-logic*: contains the formalisation of EEFF with equational logic
+- *bidirectional*: contains the formalisation of the bidirectional type inference
+
+
+All files contain `Add LoadPath` commands with the relative paths prefixed by `???` to allow a search-and-replace with the absolute path of the repository.
+
+# Predicate Logic
+
+The order of compilation is:
+1. `syntax/syntax.v`
+2. `syntax/syntax_lemmas.v`
+3. `substitution/substitution.v`
+4. `substitution/substitution_lemmas.v`
+5. `operational_semantics/operational_semantics.v`
+6. `type_system/subtyping_and_admissibility.v`
+7. `type_system/declarational.v`
+8. `type_system/wf_lemmas.v`
+9. `type_system/subtyping_lemmas.v`
+10. `logic/logic_aux_lemmas.v`
+11. `type_system/type_aux_lemmas.v`
+12. `type_system/instantiation_lemmas.v`
+13. `type_system/type_lemmas.v`
+14. `logic/logic_tactics.v`
+15. `logic/logic_lemmas.v`
+
+Locations of important proofs:
+- **Substitution lemmas** are located in `type_system/type_aux_lemmas.v` for single variable substitution and `type_system/instantiation_lemmas.v` for parallel substitution. The additional substitution lemmas for the logic are in `logic/logic_lemmas.v`
+- **Safety** is located in `type_system/type_lemmas.v`.
+- **Skeletons** and their lemmas are found in the folder`denotational_semantics`.
+- **Examples** are in the folder `examples`. This branch features the examples `pick_left`, `eta-Do`, and an outline for `generators`. Mutable state examples are on the branch `equational-logic`.
